Regex/Basic.lean
@@ -1,0 +1,49 @@
+import Batteries.Data.String
+
+namespace Regex
+
+/-!
+## Regex
+
+Definitions for Regex api
+
+-/
+
+abbrev ValidSubstring := { s : Substring // Substring.Valid s }
+abbrev ValidPos s := { pos : String.Pos // String.Pos.Valid s pos }
+
+instance instSubstringValid (s : ValidSubstring) : Inhabited (ValidPos s.val.str) where
+  default := ⟨s.val.startPos, s.property.startValid⟩
+
+instance : Coe String ValidSubstring where
+  coe s := ⟨s.toSubstring, String.valid_toSubstring s⟩
+
+/-- Represents a single match of a regex in a haystack. -/
+abbrev Match := ValidSubstring
+
+instance : ToString Match where
+  toString s :=
+    s!"'{s}', {s.val.startPos}, {s.val.stopPos}"
+
+/-- Represents the full match and capture groups for a single match in `s`. -/
+structure Captures (s : String) where
+  /-- the full match -/
+  fullMatch : Match
+  /-- the capture groups, empty groups can arise, for example, in alternatives -/
+  groups: Array (Option Match)
+  /-- `fullMatch` is a substring of `s`. -/
+  isSubstringOf : fullMatch.val.str = s
+  /-- all matches in `groups` are substrings of `s`. -/
+  areSubstringsOf : groups.all (Option.all (·.val.str = s) ·)
+
+theorem start_pos_valid_of {s : ValidSubstring} (captures : Captures s.val.str)
+    : String.Pos.Valid s.val.str captures.fullMatch.val.startPos  := by
+  have : captures.fullMatch.val.str = s.val.str := by simp [captures.isSubstringOf]
+  have := captures.fullMatch.property.startValid
+  simp_all
+
+theorem stop_pos_valid_of {s : ValidSubstring} (captures : Captures s.val.str)
+    : String.Pos.Valid s.val.str captures.fullMatch.val.stopPos  := by
+  have : captures.fullMatch.val.str = s.val.str := by simp [captures.isSubstringOf]
+  have := captures.fullMatch.property.stopValid
+  simp_all
